Dynamics for terms

theories/Statics/Value.v
@@ -7,20 +7,20 @@ Require Import Coq.Lists.List.
 Require Import Coq.Logic.Decidable.
 From Metaconfigurations.Syntax Require Import Value Ty.
 
-Reserved Notation "v :ᵥ τ" (at level 80, no associativity).
+Reserved Notation "⊢ᵥ v `: τ" (at level 80, no associativity).
 
 Inductive type : Value.t → Ty.t → Prop :=
-  | type_int (n : Z) : n :ᵥ Ty.Int
-  | type_bool (b : bool) : b :ᵥ Ty.Bool
-  | type_unit : Value.Unit :ᵥ Ty.Unit
-  | type_tuple v₁ v₂ τ₁ τ₂ : v₁ :ᵥ τ₁ → v₂ :ᵥ τ₂ → ⟨ v₁, v₂ ⟩ᵥ :ᵥ (τ₁ × τ₂)
-where "v :ᵥ τ" := (type v τ).
+  | type_int (n : Z) : ⊢ᵥ n `: Ty.Int
+  | type_bool (b : bool) : ⊢ᵥ b `: Ty.Bool
+  | type_unit : (⊢ᵥ ⊤ᵥ `: Ty.Unit)
+  | type_tuple v₁ v₂ τ₁ τ₂ : ⊢ᵥ v₁ `: τ₁ → ⊢ᵥ v₂ `: τ₂ → ⊢ᵥ ⟨ v₁, v₂ ⟩ᵥ `: (τ₁ × τ₂)
+where "⊢ᵥ v `: τ" := (type v τ).
 
-Definition with_type τ := { v | type v τ }.
+Definition with_type τ := { v | ⊢ᵥ v `: τ }.
 
 Notation "V⟦ τ ⟧" := (with_type τ).
 
-Theorem value_well_typed v : ∃ τ, v :ᵥ τ.
+Theorem value_well_typed v : ∃ τ, ⊢ᵥ v `: τ.
 Proof.
    induction v.
    - econstructor. econstructor.
@@ -29,7 +29,7 @@ Proof.
    - inversion IHv1. inversion IHv2. eexists. econstructor; eauto.
 Qed.
 
-Theorem type_deterministic v σ τ : v :ᵥ σ → v :ᵥ τ → σ = τ.
+Theorem type_deterministic v σ τ : ⊢ᵥ v `: σ → ⊢ᵥ v `: τ → σ = τ.
 Proof.
    intros Hσ. generalize dependent σ. generalize dependent τ. 
    induction v; intros; inv H; inv Hσ; try f_equal; auto.
