theories/Syntax/Stmt.v
@@ -16,11 +16,10 @@ Section Stmt.
 
   Inductive t : Type :=
     | Seq (s₁ : t) (s₂ : t)
-    | Assign (x : register_names π) (e : Term.t Π Ω)
-    | If (e : Term.t Π Ω) (s₁ : t) (s₂ : t)
-    (* | While (e : Expr.t) (s : t) *)
+    | Assign (x : register_names π) (e : Term.t Π Ω π)
+    | If (e : Term.t Π Ω π) (s₁ : t) (s₂ : t)
     | Goto (l : nat)
-    | Return (e : Term.t Π Ω)
-    | Invoke (obj : string) (op : string) (es : list (Term.t Π Ω)).
+    | Return (e : Term.t Π Ω π)
+    | Invoke (ω : Ω) (op : (type ω).(OP Π)) (arg : t).
 
 End Stmt.
